code/ecdsap256sha2/Hacl.Impl.P256.Compression.fst
@@ -9,8 +9,38 @@ open Lib.Buffer
 
 open Spec.P256.Definitions
 
+
+val eq_u8_nCT: a:uint8 -> b:uint8 -> (r:bool{r == (uint_v a = uint_v b)})
+
+let eq_u8_nCT a b =
+  let open Lib.RawIntTypes in
+  FStar.UInt8.(u8_to_UInt8 a =^ u8_to_UInt8 b)
+
+val copy_conditional_u8: out: lbuffer uint8 (size 64) -> x: lbuffer uint8 (size 64) -> mask: uint8{uint_v mask = 0 \/ uint_v mask = pow2 8 - 1} -> Stack unit 
+  (requires fun h -> live h out /\ live h x)
+  (ensures fun h0 _ h1 -> modifies (loc out) h0 h1) 
+
+let copy_conditional_u8 out x mask = 
+  ()
+
+
 let decompressionNotCompressed b result = 
-  (u64 0)
+  let compressionIdentifier = index b (size 0) in
+  let correctIdentifier = eq_u8_nCT (u8 4) compressionIdentifier in 
+  if correctIdentifier then 
+    copy (sub b (size 1) (size 64)) result;
+  admit();  
+  correctIdentifier
+
+
+let decompressionNotCompressed2 b result = 
+  let compressionIdentifier = index b (size 0) in 
+  let correctIdentifier = eq_mask (u8 4) compressionIdentifier in 
+    eq_mask_lemma (u8 4) compressionIdentifier;
+  copy_conditional_u8 result (sub b (size 1) (size 64)) correctIdentifier;
+  correctIdentifier
+
+
 
 let decompressionCompressed b result = 
   (u64 0)
