code/ecdsap256sha2/Hacl.Impl.P256.Compression.fsti
@@ -10,13 +10,23 @@ open Lib.Buffer
 open Spec.P256.Definitions
 
 
-let notCompressedForm = lbuffer uint8 (size 64)
+let notCompressedForm = lbuffer uint8 (size 65)
 let compressedForm = lbuffer uint8 (size 64)
 
 (* the name makes a lot of sense, doesnot it? *)
-val decompressionNotCompressed: notCompressedForm -> result: point -> Stack bool 
-  (requires fun h -> True)
-  (ensures fun h0 _ h1 -> True)
+
+(* the function is to decode publickey, so NOT SCA resistant *)
+
+(*void uECC_decompress(const uint8_t *compressed, uint8_t *public_key, uECC_Curve curve)  *)
+
+val decompressionNotCompressed: b: notCompressedForm -> result: lbuffer uint8 (size 64) -> Stack bool 
+  (requires fun h -> live h b /\ live h result /\ disjoint b result)
+  (ensures fun h0 _ h1 -> modifies (loc result) h0 h1)
+
+val decompressionNotCompressed2: b: notCompressedForm -> result: lbuffer uint8 (size 64) -> Stack uint8
+  (requires fun h -> live h b /\ live h result /\ disjoint b result)
+  (ensures fun h0 _ h1 -> modifies (loc result) h0 h1)
+
 
 val decompressionCompressed: compressedForm -> result: point -> Stack bool 
   (requires fun h -> True)
