code/ecdsap256sha2/Hacl.Impl.ECDSA.fsti
@@ -77,11 +77,16 @@ val ecdsa_p256_sha2_verify:
       result == Spec.ECDSA.ecdsa_verification (publicKeyX, publicKeyY) r s (v mLen) (as_seq h0 m))
 
 
+val decompressionNotCompressed: b: notCompressedForm -> result: lbuffer uint8 (size 64) -> Stack bool 
+  (requires fun h -> live h b /\ live h result)
+  (ensures fun h0 _ h1 -> modifies (loc result) h0 h1)
 
-val decompressionNotCompressed: notCompressedForm -> result: point -> Stack uint64 
+
+val decompressionCompressed: compressedForm -> result: point -> Stack bool 
   (requires fun h -> True)
   (ensures fun h0 _ h1 -> True)
 
-val decompressionCompressed: compressedForm -> result: point -> Stack uint64 
-  (requires fun h -> True)
-  (ensures fun h0 _ h1 -> True)
+
+val decompressionNotCompressed2: b: notCompressedForm -> result: lbuffer uint8 (size 64) -> Stack uint8
+  (requires fun h -> live h b /\ live h result /\ disjoint b result)
+  (ensures fun h0 _ h1 -> modifies (loc result) h0 h1)
